Wavelet/Seq/Prog.lean
@@ -17,16 +17,16 @@ open Semantics
 structure Sig where
   ι : Nat
   ω : Nat
-  -- Functions with empty inputs/outputs are not allowed
-  -- for some liveness properties
-  neZeroᵢ : NeZero ι
-  neZeroₒ : NeZero ω
-
-instance {sig : Sig} : NeZero sig.ι := sig.neZeroᵢ
-
-instance {sig : Sig} : NeZero sig.ω := sig.neZeroₒ
 
 abbrev Sigs k := Fin k → Sig
+
+/-- Signatures with non-zero arities. -/
+class NeZeroSigs (sigs : Sigs k) where
+  neZeroᵢ : ∀ i : Fin k, NeZero (sigs i).ι
+  neZeroₒ : ∀ i : Fin k, NeZero (sigs i).ω
+
+instance {sigs : Sigs k} [NeZeroSigs sigs] (i : Fin k) : NeZero (sigs i).ι := NeZeroSigs.neZeroᵢ i
+instance {sigs : Sigs k} [NeZeroSigs sigs] (i : Fin k) : NeZero (sigs i).ω := NeZeroSigs.neZeroₒ i
 
 inductive SigOps (sigs : Sigs k) (k' : Fin (k + 1)) where
   | call (i : Fin k')
@@ -46,8 +46,10 @@ def SigOps.elim0 : SigOps sigs ⟨0, by simp⟩ → α
 instance : Arity (SigOps sigs k') where
   ι | .call i => (sigs ↓i).ι
   ω | .call i => (sigs ↓i).ω
-  neZeroᵢ | .call i => (sigs ↓i).neZeroᵢ
-  neZeroₒ | .call i => (sigs ↓i).neZeroₒ
+
+instance [NeZeroSigs sigs] : NeZeroArity (SigOps sigs k') where
+  neZeroᵢ | .call i => by apply NeZeroSigs.neZeroᵢ
+  neZeroₒ | .call i => by apply NeZeroSigs.neZeroₒ
 
 abbrev Prog (Op : Type u) χ V [Arity Op] (sigs : Sigs k) :=
   (i : Fin k) → Fn (Op ⊕ SigOps sigs i.castSucc) χ V (sigs i).ι (sigs i).ω
